characteristic/cfTacticsLib.sml
@@ -96,7 +96,7 @@ fun cf_get_precondition t = rand (rator t)
 (* xx *)
 val cf_defs =
   [cf_lit_def, cf_con_def, cf_var_def, cf_let_def, cf_opn_def, cf_opb_def,
-   cf_app_def, cf_fundecl_def, cf_fundecl_rec_def, cf_ref_def, cf_assign_def,
+   cf_app_def, cf_fun_def, cf_fun_rec_def, cf_ref_def, cf_assign_def,
    cf_deref_def, cf_aalloc_def, cf_asub_def, cf_alength_def, cf_aupdate_def,
    cf_aw8alloc_def, cf_aw8sub_def, cf_aw8length_def, cf_aw8update_def,
    cf_log_def, cf_if_def, cf_match_def]
@@ -224,7 +224,7 @@ val reduce_spec_conv =
 
 val reduce_curried_conv = RATOR_CONV (RAND_CONV eval)
 
-val fundecl_reduce_conv =
+val fun_reduce_conv =
   QUANT_CONV (
     LAND_CONV (
       LAND_CONV reduce_curried_conv THENC
@@ -232,9 +232,9 @@ val fundecl_reduce_conv =
     )
   )
 
-fun fundecl_rec_aux_unfold_conv tm = let
-  val base_case = fst (CONJ_PAIR fundecl_rec_aux_def)
-  val ind_case = fst (CONJ_PAIR (snd (CONJ_PAIR fundecl_rec_aux_def)))
+fun fun_rec_aux_unfold_conv tm = let
+  val base_case = fst (CONJ_PAIR fun_rec_aux_def)
+  val ind_case = fst (CONJ_PAIR (snd (CONJ_PAIR fun_rec_aux_def)))
   val base_conv = REWR_CONV base_case
   val ind_conv =
     REWR_CONV ind_case THENC
@@ -243,11 +243,11 @@ fun fundecl_rec_aux_unfold_conv tm = let
       RAND_CONV reduce_spec_conv
     ) THENC
     RAND_CONV (
-      fundecl_rec_aux_unfold_conv
+      fun_rec_aux_unfold_conv
     )
 in (base_conv ORELSEC ind_conv) tm end
 
-val fundecl_rec_reduce_conv = let
+val fun_rec_reduce_conv = let
   val reduce_length =
       eval THENC
       simp_conv [LENGTH_EQ_NUM_compute, PULL_EXISTS]
@@ -263,24 +263,24 @@ in
     )
   ) THENC
   simp_conv [PULL_EXISTS] THENC
-  QUANT_CONV fundecl_rec_aux_unfold_conv
+  QUANT_CONV fun_rec_aux_unfold_conv
 end
 
 val xfun_norec_core =
-  head_unfold cf_fundecl_def \\
+  head_unfold cf_fun_def \\
   irule local_elim \\ hnf \\
-  CONV_TAC fundecl_reduce_conv
+  CONV_TAC fun_reduce_conv
 
 val xfun_rec_core =
-  head_unfold cf_fundecl_rec_def \\
+  head_unfold cf_fun_rec_def \\
   irule local_elim \\ hnf \\
-  CONV_TAC fundecl_rec_reduce_conv
+  CONV_TAC fun_rec_reduce_conv
 
 fun xfun qname =
   xpull_check_not_needed \\
   first_match_tac [
-    ([mg.c `cf_fundecl _ _ _ _ _ _ _ _`], K xfun_norec_core),
-    ([mg.c `cf_fundecl_rec _ _ _ _ _ _`], K xfun_rec_core)
+    ([mg.c `cf_fun _ _ _ _ _ _ _ _`], K xfun_norec_core),
+    ([mg.c `cf_fun_rec _ _ _ _ _ _`], K xfun_rec_core)
   ] \\
   qx_gen_tac qname \\
   rpt strip_tac
